src/mulx/Curve25519_Hop4.ec
@@ -4,19 +4,19 @@ require import Curve25519_Spec.
 require import Curve25519_Hop1.
 require import Curve25519_Hop2.
 require import Curve25519_Hop3.
-require import Curve25519_ref4.
-require import Curve25519_auto.
+require import Curve25519_Ref4.
+require import Curve25519_auto_mulx.
 require import W64limbs.
 import Zp_25519.
-import Curve25519_Spec Curve25519_auto Curve25519_Hop1 Curve25519_Hop2 Curve25519_ref4 Array4 Array8 Array32 StdOrder.IntOrder.
+import Curve25519_Spec Curve25519_auto_mulx Curve25519_Hop1 Curve25519_Hop2 Curve25519_mulx Array4 Array8 Array32 StdOrder.IntOrder.
 
 
 (* Should be moved elsewhere *)
 
 (** init **)
 
-equiv eq_h4_init_points :
-    MHop2.init_points ~ M.__init_points4 : 
+equiv eq_h4_init_points_mulx :
+    MHop2.init_points ~ M_mulx.__init_points4 : 
         init{1} = inzpRep4 initr{2}
         ==> 
         res{1}.`1 = inzpRep4 res{2}.`1 /\
@@ -33,8 +33,8 @@ proof.
     rewrite /H6  /H0 /H3 /H2 /Zp_25519.zero /set0_64_ /inzpRep4 // /valRep4 /to_list /mkseq -iotaredE  => />.
 qed. 
 
-equiv eq_h4_decode_u_coordinate_base :
-    MHop2.decode_u_coordinate_base ~ M.__decode_u_coordinate_base4:
+equiv eq_h4_decode_u_coordinate_base_mulx :
+    MHop2.decode_u_coordinate_base ~ M_mulx.__decode_u_coordinate_base4:
         true 
         ==> 
         res{1} = inzpRep4 res{2}.
@@ -45,8 +45,8 @@ qed.
 
 
 (** step 4 : cswap **)
-equiv eq_h4_cswap :
-    MHop2.cswap ~ M.__cswap4:
+equiv eq_h4_cswap_mulx :
+    MHop2.cswap ~ M_mulx.__cswap4:
         x2{1}         = inzpRep4 x2{2}      /\
         z2{1}         = inzpRep4 z2r{2}     /\
         x3{1}         = inzpRep4 x3{2}      /\
@@ -82,8 +82,8 @@ proof.
 qed.
 
 (** step 5 : add_and_double **)
-equiv eq_h4_add_and_double :
-    MHop2.add_and_double ~ M.__add_and_double4:
+equiv eq_h4_add_and_double_mulx :
+    MHop2.add_and_double ~ M_mulx.__add_and_double4:
         init{1} = inzpRep4 init{2}     /\
         x2{1}   = inzpRep4 x2{2}       /\
         z2{1}   = inzpRep4 z2r{2}      /\
@@ -96,30 +96,18 @@ equiv eq_h4_add_and_double :
         res{1}.`4 = inzpRep4 res{2}.`4.
 proof.
     proc => /=.
-    call eq_h4_mul_rss.
-    call eq_h4_mul_sss.
-    call eq_h4_add_sss.
-    call eq_h4_sqr_ss_.
-    call eq_h4_mul_a24_ss.
-    call eq_h4_sqr_ss_.
-    call eq_h4_sub_sss.
-    call eq_h4_mul_sss.
-    call eq_h4_sub_sss.
-    call eq_h4_add_sss.
-    call eq_h4_sqr_ss_.
-    call eq_h4_sqr_ss_.
-    call eq_h4_mul_sss.
-    call eq_h4_mul_sss.
-    call eq_h4_add_sss.
-    call eq_h4_sub_sss.
-    call eq_h4_add_ssr.
-    call eq_h4_sub_ssr.
-    wp. done.
+    call eq_h4_mul_rss_mulx.
+    call eq_h4_mul_sss_mulx.
+    call eq_h4_add_sss_mulx.
+    call eq_h4_sqr_ss_mulx.
+    call eq_h4_mul_a24_ss_mulx.
+    call eq_h4_sqr_ss_mulx.
+    admit.
 qed.
 
 (** step 6 : montgomery_ladder_step **)
-equiv eq_h4_montgomery_ladder_step :
-    MHop2.montgomery_ladder_step ~ M.__montgomery_ladder_step4:
+equiv eq_h4_montgomery_ladder_step_mulx :
+    MHop2.montgomery_ladder_step ~ M_mulx.__montgomery_ladder_step4:
         inzp (to_uint k'{1}) =   inzpRep32 k{2} /\
         init'{1} = inzpRep4 init{2}             /\
         x2{1} = inzpRep4 x2{2}                  /\
@@ -136,9 +124,9 @@ equiv eq_h4_montgomery_ladder_step :
         b2i res{1}.`5 = to_uint res{2}.`5.
 proof.
     proc => /=. 
-    call eq_h4_add_and_double. wp.
-    call eq_h4_cswap. wp.
-    call eq_h4_ith_bit. skip. 
+    call eq_h4_add_and_double_mulx. wp.
+    call eq_h4_cswap_mulx. wp.
+    call eq_h4_ith_bit_mulx. skip. 
     move => &1 &2 [H0] [H1] [H2] [H3] [H4] [H5] [H6] H7. split.   
     auto => />. rewrite H0. 
     move => [H8 H9] H10 H11 H12 H13 H14. 
@@ -150,8 +138,8 @@ proof.
 qed.   
 
 (** step 7 : montgomery_ladder **)
-equiv eq_h4_montgomery_ladder :
-    MHop2.montgomery_ladder ~ M.__montgomery_ladder4 :
+equiv eq_h4_montgomery_ladder_mulx :
+    MHop2.montgomery_ladder ~ M_mulx.__montgomery_ladder4 :
         init'{1} = inzpRep4 u{2}                     /\
         inzp (W256.to_uint k'{1}) =  inzpRep32 k{2}
         ==>
@@ -165,26 +153,25 @@ proof.
     while(
           inzp (to_uint k'{1}) = inzpRep32 k{2}            /\ 
           ctr{1} = to_uint ctr{2}                          /\ 
-          inzp (to_uint k'{1}) = inzpRep32 k{2}            /\
           init'{1} = inzpRep4 us{2}                        /\ 
           x2{1} = inzpRep4 x2{2}                           /\
           x3{1} = inzpRep4 x3{2}                           /\
           z2{1} = inzpRep4 z2r{2}                          /\
           z3{1} = inzpRep4 z3{2}                           /\
           b2i swapped{1} = to_uint swapped{2}).
-        wp. sp. call eq_h4_montgomery_ladder_step. skip. auto => />. 
+        wp. sp. call eq_h4_montgomery_ladder_step_mulx. skip. auto => />. 
         move => &1 &2 ctrR H H0 H1 H2. split.
         rewrite to_uintB. rewrite uleE to_uint1 => />. smt(). rewrite to_uint1 => />.
         move => H3 H4 H5 H6 H7 H8 H9 H10. split.
         rewrite ultE to_uintB. rewrite uleE to_uint1. smt().
         rewrite to_uint1 to_uint0. trivial. smt(@W64).  
-    call eq_h4_montgomery_ladder_step. wp. call eq_h4_init_points. skip. done.
+    call eq_h4_montgomery_ladder_step_mulx. wp. call eq_h4_init_points_mulx. skip. done.
 qed.
 
 (** step 8 : iterated square **)
-equiv eq_h4_it_sqr :
-    MHop2.it_sqr ~ M._it_sqr4_p:
-        f{1}            =    inzpRep4 x{2} /\
+equiv eq_h4__it_sqr_x2_mulx :
+    MHop2.it_sqr_x2 ~ M_mulx.__it_sqr4_x2:
+         f{1}            =    inzpRep4 f{2} /\
         i{1}            =    to_uint i{2}  /\
         2               <=   to_uint i{2}  /\
         i{1}            <=   W32.modulus   /\
@@ -193,42 +180,46 @@ equiv eq_h4_it_sqr :
         res{1} = inzpRep4 res{2}.
 proof.
     proc. simplify. wp. sp.
-    while (h{1}            =    inzpRep4 x{2}            /\ 
+    while (h{1}            =    inzpRep4 h{2}            /\ 
+         f{1}             = inzpRep4 f{2} /\
          ii{1}            =    to_uint i{2}              /\
          ii{1}            <=   W32.modulus               /\
          0                <=   ii{1}                     
     ).
-    wp. call eq_h4_sqr_p. conseq(_: _ ==> h{1} = inzpRep4 x{2}).
-    move => &1 &2 [[H][ H0] [H1] H2 [H3] H4 H5]. split. apply H5.
+    wp. sp. call eq_h4_sqr__rr_mulx.  call eq_h4_sqr__rr_mulx. 
+    conseq(_: _ ==> f{1} = inzpRep4 f{2} /\  h{1} = inzpRep4 h{2}).
     rewrite /DEC_32 /rflags_of_aluop_nocf_w /ZF_of => /=.
-    move => H6 H7 H8 H9. split. split. apply H9. split.
-    rewrite to_uintB. rewrite  uleE => />. by smt(). rewrite to_uint1 H0 //.
-    split. move: H1. smt(). move: H2. smt(). split. rewrite H0. move => H10.
-    smt(@W32). smt(@W32). skip. auto => />. wp.
+    move=> &1 &2 [H1 [[H2]] [H3] [H4] [H5] H6 [H7] H8 [H9] H10]. split. apply H9.
+    move => H11 H12 H13 H14. split. apply H14. move => H15 H16 H17 H18.
+    split. split. rewrite H14. trivial. split. apply H18. split.
+    rewrite H1. rewrite to_uintB. rewrite  uleE => />. smt(). rewrite to_uint1 H4 //.
+    split. move: H5. smt(). move: H7. smt(). split. move => H19.
+    rewrite H1. smt(@W32). rewrite H1. smt(@W32).  
+    skip. auto => />. 
+    wp. call eq_h4_sqr__rr_mulx.  call eq_h4_sqr__rr_mulx. 
     rewrite /DEC_32 /rflags_of_aluop_nocf_w /ZF_of => /=. 
-    call eq_h4_sqr_p.  
-    skip. auto => />. move => &2 H H0. split. split.
+    auto => />. move => &2 H H0. split. split. 
     rewrite to_uintB. rewrite uleE => />. move: H. smt().
     rewrite to_uint1 //. split. move: H0. smt(). move: H. smt().
-    split. move => H1. smt(@W32). move => H1. move: H. smt().
+    split. move => H3. smt(@W32). move => H4. move: H. smt().    
 qed.
 
-equiv eq_h4_it_sqr_s :
-    MHop2.it_sqr ~ M._it_sqr4_s_:
-        f{1}            =    inzpRep4 x{2} /\
+equiv eq_h4_it_sqr_x2_mulx :
+    MHop2.it_sqr_x2 ~ M_mulx._it_sqr4_x2:
+        f{1}            =    inzpRep4 f{2} /\
         i{1}            =    to_uint i{2}  /\
         2               <=   to_uint i{2}  /\
         i{1}            <=   W32.modulus   /\
         2              <=   i{1}   ==>
         res{1} = inzpRep4 res{2}.
 proof.
-    proc *. inline M._it_sqr4_s_. wp. sp. 
-    call eq_h4_it_sqr. skip. auto => />.
+    proc *. inline M_mulx._it_sqr4_x2. wp. sp. 
+    call eq_h4__it_sqr_x2_mulx. skip. auto => />.
 qed.
 
-equiv eq_h4_it_sqr_ss :
-        MHop2.it_sqr ~ M._it_sqr4_ss_: 
-        f{1}            =    inzpRep4 x{2} /\
+equiv eq_h4_it_sqr_x2__mulx :
+        MHop2.it_sqr_x2 ~ M_mulx._it_sqr4_x2_: 
+        f{1}            =    inzpRep4 _f{2} /\
         i{1}            =    to_uint i{2}  /\
         2               <=   to_uint i{2}  /\
         i{1}            <=   W32.modulus   /\
@@ -236,67 +227,43 @@ equiv eq_h4_it_sqr_ss :
         ==>
         res{1} = inzpRep4 res{2}.
 proof.
-    proc *. inline M._it_sqr4_ss_. 
-    unroll for{2} ^while. wp. sp.
-    call eq_h4_it_sqr. skip. auto => />. move => &2 H H0. congr. 
-    apply Array4.ext_eq. move => H1 [H2] H3. smt(@Array4).
+    proc *. inline M_mulx._it_sqr4_x2_. 
+    wp. sp. call eq_h4_it_sqr_x2_mulx. skip.
+    auto => />.
 qed.
 
 (** step 9 : invert **)
-equiv eq_h4_invert :
-    MHop2.invert ~ M.__invert4 : 
-        fs{1} = inzpRep4 fs{2}
+equiv eq_h4_invert_mulx :
+    MHop2.invert ~ M_mulx.__invert4 : 
+        fs{1} = inzpRep4 f{2}
         ==> 
         res{1} = inzpRep4 res{2}.
 proof.
     proc.
     sp.
-    call eq_h4_mul_ss.
-    call eq_h4_sqr_s_.
-    call (eq_h4_it_sqr_s). wp.
-    call eq_h4_mul_ss.
-    call eq_h4_it_sqr_s. wp.
-    call eq_h4_mul_ss.
-    call eq_h4_it_sqr_ss. wp.
-    call eq_h4_mul_ss.
-    call eq_h4_it_sqr_ss. wp.
-    call eq_h4_mul_ss.
-    call eq_h4_it_sqr_s. wp.
-    call eq_h4_mul_ss.
-    call eq_h4_it_sqr_ss. wp.
-    call eq_h4_mul_ss.
-    call eq_h4_it_sqr_ss. wp.
-    call eq_h4_mul_ss.
-    call eq_h4_it_sqr_s. wp.
-    call eq_h4_sqr_ss.
-    call eq_h4_mul_ss.
-    call eq_h4_sqr_ss.
-    call eq_h4_mul_ss.
-    call eq_h4_mul_ss.
-    call eq_h4_sqr_s_.
-    call eq_h4_sqr_ss.
-    call eq_h4_sqr_ss. wp. 
-    skip. done.
+    call eq_h4_mul_rsr__mulx.
+    call eq_h4_sqr_rr_mulx.
+    admit.
 qed.
 
 
 (** step 11 : scalarmult **)
 
-equiv eq_h4_scalarmult_internal :
-    MHop2.scalarmult_internal ~ M.__curve25519_internal_ref4:
+equiv eq_h4_scalarmult_internal_mulx :
+    MHop2.scalarmult_internal ~ M_mulx.__curve25519_internal_mulx:
         inzp(W256.to_uint k'{1}) = inzpRep32 k{2} /\  
         u''{1} = inzpRep4 u{2}
         ==>
         inzp(W256.to_uint res{1}) = inzpRep4 res{2}. 
 proof.
     proc.
-    call eq_h4_encode_point.
-    call eq_h4_montgomery_ladder. wp. skip.
+    call eq_h4_encode_point_mulx.
+    call eq_h4_montgomery_ladder_mulx. wp. skip.
     done.
 qed.
 
-equiv eq_h4_scalarmult :
-    MHop2.scalarmult ~ M._curve25519_ref4:
+equiv eq_h4_scalarmult_mulx :
+    MHop2.scalarmult ~ M_mulx.__curve25519_mulx:
         inzp(W256.to_uint k'{1}) = inzpRep4 _k{2} /\  
         inzp (to_uint u'{1}) = inzpRep4 _u{2}
         ==>
@@ -304,13 +271,13 @@ equiv eq_h4_scalarmult :
         inzpRep32List (W32u8.to_list res{1}) = inzpRep4 res{2}.
 proof.
     proc.
-    call eq_h4_scalarmult_internal => />. auto => />.
+    call eq_h4_scalarmult_internal_mulx => />. auto => />.
     move => &1 &2 H H0 H1 H2 H3 H4 H5 H6 H7. auto => />.
     rewrite -H7.
     rewrite /inzpRep32List /inzpRep4 /valRep32List. congr. 
     rewrite to_uint_unpack32u8. congr. congr. smt().
-    call eq_h4_decode_u_coordinate => />.
-    call eq_h4_decode_scalar_25519 => />.
+    call eq_h4_decode_u_coordinate_mulx => />.
+    call eq_h4_decode_scalar_25519_mulx => />.
     move => &1 &2 [H] H0 H1. split. auto => />.
     move => H2 H3 H4 H5 H6. split. auto => />.
     move => H7 H8 H9 H10. rewrite -H10.
@@ -323,95 +290,21 @@ proof.
     rewrite to_uint_unpack32u8. congr. congr. smt().
 qed.
 
-
-lemma eq_h4_scalarmult_ptr mem _rp _kp _up :
-    equiv [MHop2.scalarmult ~ M.__curve25519_ref4_ptr:
-        valid_ptr (W64.to_uint _up)  32                                                          /\ 
-        valid_ptr (W64.to_uint _kp)  32                                                          /\
-        valid_ptr (W64.to_uint _rp)  32                                                          /\
-        Glob.mem{2} = mem                                                                        /\
-        rp{2} = _rp                                                                              /\ 
-        kp{2} = _kp                                                                              /\
-        up{2} = _up                                                                              /\ 
-        inzp (W256.to_uint u'{1}) = inzpRep4List (load_array4 (mem) (W64.to_uint _up))           /\
-        inzp (W256.to_uint k'{1}) = inzpRep4List (load_array4 (mem) (W64.to_uint _kp))             
-        ==>
-        inzpRep32List(W32u8.to_list res{1}) = inzpRep4List (load_array4 Glob.mem{2} (W64.to_uint _rp))    /\
-        res{2} = tt
-    ].
-proof.
-    proc *.
-    inline M.__curve25519_ref4_ptr. wp. sp.
-    inline M.__load4 M.__store4. 
-    do 3! unroll for{2} ^while.
-    sp. wp. auto => />.
-    call eq_h4_scalarmult. skip. auto => />.
-    move => &1 &2 H H0 H1 H2 H3 H4 H5 H6. 
-    split. split.
-    rewrite H6 /inzpRep4List /inzpRep4 /valRep4 /valRep4List /load_array4.
-    congr. congr. congr. rewrite /to_list /mkseq -iotaredE. auto => />.  
-    rewrite !to_uintD_small !to_uint_small => />. 
-    move: H2. smt(). move: H1. smt(). move: H2. smt().
-    rewrite H5 /inzpRep4List /inzpRep4 /valRep4 /valRep4List /load_array4.
-    congr. congr. congr. rewrite /to_list /mkseq -iotaredE. auto => />.  
-    rewrite !to_uintD_small !to_uint_small => />. 
-    move: H5. smt(). move: H5. smt(). move: H5. smt().
-    move => H7 H8 H9 H10 H11. auto => />. rewrite -H11.
-    move => H12. rewrite H12 H11.
-    rewrite /inzpRep4List /inzpRep4 /valRep4 /valRep4List /load_array4.
-    congr. congr. congr. rewrite /to_list /mkseq -iotaredE => />. 
-    split. apply (load_store_pos Glob.mem{2} rp{2} H10 0). 
-    rewrite /valid_ptr. split. trivial. apply H4. trivial.
-    split. apply (load_store_pos Glob.mem{2} rp{2} H10 8). 
-    rewrite /valid_ptr. split. trivial. apply H4. trivial.
-    split. apply (load_store_pos Glob.mem{2} rp{2} H10 16). 
-    rewrite /valid_ptr. split. trivial. apply H4. trivial.
-    apply (load_store_pos Glob.mem{2} rp{2} H10 24). 
-    rewrite /valid_ptr. split. trivial. apply H4. trivial.    
-qed.
-
-
-equiv eq_h4_scalarmult_base :
-    MHop2.scalarmult_base ~ M._curve25519_ref4_base:
+equiv eq_h4_scalarmult_base_mulx :
+    MHop2.scalarmult_base ~ M_mulx.__curve25519_mulx_base:
         inzp(W256.to_uint k'{1}) = inzpRep4 _k{2} 
         ==>  
         inzp(W256.to_uint res{1}) = inzpRep4 res{2}. 
 proof.
     proc.
-    call eq_h4_scalarmult_internal => />.
-    call eq_h4_decode_u_coordinate_base => />.
-    call eq_h4_decode_scalar_25519.
+    call eq_h4_scalarmult_internal_mulx => />.
+    call eq_h4_decode_u_coordinate_base_mulx => />.
+    call eq_h4_decode_scalar_25519_mulx.
     wp. skip. done.
 qed.
 
-
-lemma eq_h4_scalarmult_base_ptr mem _rp _kp : 
- equiv [MHop2.scalarmult_base ~ M.__curve25519_ref4_base_ptr:
-        valid_ptr (W64.to_uint _rp) 32 /\
-        valid_ptr (W64.to_uint _kp) 32 /\
-        Glob.mem{2} = mem /\
-        rp{2} = _rp /\
-        kp{2} = _kp /\
-        inzp(W256.to_uint k'{1}) = inzpRep4List (load_array4 (Glob.mem{2}) (W64.to_uint _kp))
-        ==>
-        inzp(W256.to_uint res{1}) = inzpRep4List (load_array4 Glob.mem{2} (W64.to_uint _rp)) /\ res{2} = tt].
-proof.
-    proc *. inline M.__curve25519_ref4_base_ptr M.__load4 M.__store4. 
-    do 2! unroll for{2} ^while. wp. sp. call eq_h4_scalarmult_base.
-    skip. auto => />.  move => &1 &2 H H0 H1 H2. split.
-    rewrite H2. rewrite /inzpRep4List /inzpRep4 /valRep4 /valRep4List /load_array4 /to_list /mkseq -iotaredE.
-    congr. congr. congr. auto => />. rewrite !to_uintD_small !to_uint_small; smt(); smt().    
-    move => H3 H4 H5 H6. rewrite H6. rewrite /inzpRep4 /inzpRep4List /valRep4 /valRep4List.
-    congr. congr. congr. rewrite /to_list /mkseq /load_array4 -iotaredE => />. split.
-    apply (load_store_pos mem _rp H5 0). rewrite /valid_ptr. smt(). smt(). split.
-    apply (load_store_pos mem _rp H5 8). rewrite /valid_ptr. smt(). smt(). split.
-    apply (load_store_pos mem _rp H5 16). rewrite /valid_ptr. smt(). smt(). 
-    apply (load_store_pos mem _rp H5 24). rewrite /valid_ptr. smt(). smt().
-qed.    
-
-
-lemma eq_h4_scalarmult_jade mem _qp _np _pp:
-    equiv [MHop2.scalarmult ~ M.jade_scalarmult_curve25519_amd64_ref4:
+lemma eq_h4_scalarmult_jade_mulx mem _qp _np _pp:
+    equiv [MHop2.scalarmult ~ M_mulx.jade_scalarmult_curve25519_amd64_mulx:
         valid_ptr (W64.to_uint _qp)  32                                                          /\ 
         valid_ptr (W64.to_uint _np)  32                                                          /\
         valid_ptr (W64.to_uint _pp)  32                                                          /\
@@ -425,16 +318,33 @@ lemma eq_h4_scalarmult_jade mem _qp _np _pp:
         inzp(W256.to_uint res{1}) = inzpRep4List (load_array4 Glob.mem{2} (W64.to_uint _qp))     /\
         res{2} = W64.zero].
 proof.
-    proc *. inline M.jade_scalarmult_curve25519_amd64_ref4. wp. sp.
-    call (eq_h4_scalarmult_ptr mem _qp _np _pp). skip. auto => />.
-    move => &1 H H0 H1 H2 H3 H4 H5 H6 H7 H8 H9.
-    rewrite -H9. rewrite to_uint_unpack32u8. rewrite /inzpRep32List /valRep32List.
-    congr. congr. congr. smt(@W32u8).
+    proc *. inline M_mulx.jade_scalarmult_curve25519_amd64_mulx. wp. sp.
+    inline M_mulx.__load4 M_mulx.__store4. 
+    do 3! unroll for{2} ^while. wp. sp.
+    call eq_h4_scalarmult_mulx. skip. auto => />.
+    move => &1 &2 H H0 H1 H2 H3 H4 H5 H6. split. split.
+    rewrite H5. rewrite /inzpRep4List /inzpRep4 /inzpRep4 /valRep4 /valRep4List /load_array4.
+    congr. congr. congr. rewrite /to_list /mkseq -iotaredE => />. split. 
+    rewrite !to_uintD_small !to_uint_small. move: H2. auto => />. smt(). auto => />.
+    trivial. split.     rewrite !to_uintD_small !to_uint_small. move: H2. auto => />. smt(). auto => />.
+    trivial. rewrite !to_uintD_small !to_uint_small. move: H2. auto => />. smt(). auto => />.
+    trivial. rewrite !to_uintD_small !to_uint_small. move: H2. auto => />. smt(). auto => />.
+    trivial. smt(). trivial. smt(). trivial. smt(). smt().
+    rewrite H6. rewrite /inzpRep4List /inzpRep4 /inzpRep4 /valRep4 /valRep4List /load_array4.
+    congr. congr. congr. rewrite /to_list /mkseq -iotaredE => />. 
+    move => H7 H8 H9 H10 H11 H12. 
+    rewrite H11. rewrite /inzpRep4List /inzpRep4 /valRep4List /valRep4.
+    congr. congr. congr. rewrite /to_list /mkseq -iotaredE => />. rewrite /load_array4 => />.
+    split. 
+    apply (load_store_pos Glob.mem{2} qp{2} H10 0). rewrite /valid_ptr. split. trivial. apply H0. trivial. split.
+    apply (load_store_pos Glob.mem{2} qp{2} H10 8). rewrite /valid_ptr. split. trivial. apply H0. trivial. split.
+    apply (load_store_pos Glob.mem{2} qp{2} H10 16). rewrite /valid_ptr. split. trivial. apply H0. trivial.    
+    apply (load_store_pos Glob.mem{2} qp{2} H10 24). rewrite /valid_ptr. split. trivial. apply H0. trivial.   
 qed.
 
 
 lemma eq_h4_scalarmult_jade_base  mem _qp _np:
-    equiv [MHop2.scalarmult_base ~ M.jade_scalarmult_curve25519_amd64_ref4_base:
+    equiv [MHop2.scalarmult_base ~ M_mulx.jade_scalarmult_curve25519_amd64_mulx_base:
         valid_ptr (W64.to_uint _qp)  32                                                          /\ 
         valid_ptr (W64.to_uint _np)  32                                                          /\
         Glob.mem{2} = mem                                                                        /\
@@ -445,8 +355,26 @@ lemma eq_h4_scalarmult_jade_base  mem _qp _np:
         inzp(W256.to_uint res{1}) = inzpRep4List (load_array4 Glob.mem{2} (W64.to_uint _qp))     /\
         res{2} = W64.zero].
 proof.
-    proc *. inline M.jade_scalarmult_curve25519_amd64_ref4_base. wp. sp.
-    call (eq_h4_scalarmult_base_ptr mem _qp _np). skip. done.
+     proc *. inline M_mulx.jade_scalarmult_curve25519_amd64_mulx_base. wp. sp.
+    inline M_mulx.__load4 M_mulx.__store4. 
+    do 2! unroll for{2} ^while. wp. sp.
+    call eq_h4_scalarmult_base_mulx. skip. auto => />.
+    move => &1 &2 H H0 H1 H2 H3. split. 
+    rewrite H3. rewrite /inzpRep4List /inzpRep4 /inzpRep4 /valRep4 /valRep4List /load_array4.
+    congr. congr. congr. rewrite /to_list /mkseq -iotaredE => />.  split. 
+    rewrite !to_uintD_small !to_uint_small => />. move: H2. smt(). split.
+    rewrite !to_uintD_small !to_uint_small => />. move: H2. smt(). 
+    rewrite !to_uintD_small !to_uint_small => />. move: H2. smt().
+    move => H4 H5 H6 H7. 
+    rewrite H7. rewrite /inzpRep4List /inzpRep4 /valRep4List /valRep4.
+    congr. congr. congr. rewrite /to_list /mkseq -iotaredE => />.  rewrite /load_array4 => />.
+    split. 
+    apply (load_store_pos Glob.mem{2} qp{2} H6 0). rewrite /valid_ptr. split. trivial. apply H0. trivial. 
+    split.
+    apply (load_store_pos Glob.mem{2} qp{2} H6 8). rewrite /valid_ptr. split. trivial. apply H0. trivial. 
+    split.
+    apply (load_store_pos Glob.mem{2} qp{2} H6 16). rewrite /valid_ptr. split. trivial. apply H0. trivial.    
+    apply (load_store_pos Glob.mem{2} qp{2} H6 24). rewrite /valid_ptr. split. trivial. apply H0. trivial.   
 qed.
 
 
