src/ref4/Curve25519_Hop4.ec
@@ -1,0 +1,453 @@
+require import AllCore Bool List Int IntDiv StdOrder CoreMap Real Zp_25519 Ring EClib Distr.
+from Jasmin require import JModel JMemory JWord.
+require import Curve25519_Spec.
+require import Curve25519_Hop1.
+require import Curve25519_Hop2.
+require import Curve25519_Hop3.
+require import Curve25519_Ref4.
+require import Curve25519_auto4.
+require import W64limbs.
+import Zp_25519.
+import Curve25519_Spec Curve25519_auto4 Curve25519_Hop1 Curve25519_Hop2 Curve25519_Ref4 Array4 Array8 Array32 StdOrder.IntOrder.
+
+
+(* Should be moved elsewhere *)
+
+(** init **)
+
+equiv eq_h4_init_points_ref4 :
+    MHop2.init_points ~ M_ref4.__init_points4 : 
+        init{1} = inzpRep4 initr{2}
+        ==> 
+        res{1}.`1 = inzpRep4 res{2}.`1 /\
+        res{1}.`2 = inzpRep4 res{2}.`2 /\
+        res{1}.`3 = inzpRep4 res{2}.`3 /\
+        res{1}.`4 = inzpRep4 res{2}.`4.
+proof.
+    proc. 
+    wp. unroll for{2} ^while. wp. skip. move => &1 &2 H H0 H1 H2 H3 H4 H5 H6.
+    split; auto => />. rewrite /H4 /H0 /H2 /H3 /Zp_25519.one /set0_64_ /inzpRep4 => />.
+        rewrite /valRep4 /to_list /mkseq -iotaredE => />.
+    split; auto => />. rewrite /H5  /H0 /H3 /H2 /Zp_25519.zero /set0_64_ /inzpRep4 => />.
+        rewrite /valRep4 /to_list /mkseq -iotaredE  => />.
+    rewrite /H6  /H0 /H3 /H2 /Zp_25519.zero /set0_64_ /inzpRep4 // /valRep4 /to_list /mkseq -iotaredE  => />.
+qed. 
+
+equiv eq_h4_decode_u_coordinate_base_ref4 :
+    MHop2.decode_u_coordinate_base ~ M_ref4.__decode_u_coordinate_base4:
+        true 
+        ==> 
+        res{1} = inzpRep4 res{2}.
+proof.
+    proc. wp. skip. move => &1 &2 H.
+    rewrite /inzpRep4. congr. rewrite /valRep4 /to_list /mkseq -iotaredE => />.
+qed.
+
+
+(** step 4 : cswap **)
+equiv eq_h4_cswap_ref4 :
+    MHop2.cswap ~ M_ref4.__cswap4:
+        x2{1}         = inzpRep4 x2{2}      /\
+        z2{1}         = inzpRep4 z2r{2}     /\
+        x3{1}         = inzpRep4 x3{2}      /\
+        z3{1}         = inzpRep4 z3{2}      /\
+        b2i toswap{1} = to_uint toswap{2}
+        ==>
+        res{1}.`1     = inzpRep4 res{2}.`1  /\
+        res{1}.`2     = inzpRep4 res{2}.`2  /\
+        res{1}.`3     = inzpRep4 res{2}.`3  /\
+        res{1}.`4     = inzpRep4 res{2}.`4.
+proof.
+    proc.
+    do 4! unroll for{2} ^while.
+    case: (toswap{1}).
+        rcondt {1} 1 => //. wp => /=. skip.
+        move => &1 &2 [#] 4!->> ??.
+        have mask_set :  (set0_64.`6 - toswap{2}) = W64.onew. rewrite /set0_64_ /=. smt(@W64).
+        rewrite !mask_set /=.
+        have lxor1 : forall (x1 x2:W64.t),  x1 `^` (x2 `^` x1) = x2.
+            move=> *. rewrite xorwC -xorwA xorwK xorw0 //.
+        have lxor2 : forall (x1 x2:W64.t),  x1 `^` (x1 `^` x2) = x2.
+            move=> *. rewrite xorwA xorwK xor0w //. 
+        rewrite !lxor1 !lxor2.
+        split. congr. apply Array4.ext_eq. smt(@Array4).
+        split. congr. apply Array4.ext_eq. smt(@Array4).
+        split. congr. apply Array4.ext_eq. smt(@Array4).
+        congr. apply Array4.ext_eq. smt(@Array4).
+    rcondf {1} 1 => //. wp => /=; skip.
+    move => &1 &2 [#] 4!->> ??.
+    have mask_not_set :  (set0_64.`6 - toswap{2}) = W64.zero. smt(@W64).
+    rewrite !mask_not_set !andw0 !xorw0.
+    smt(@Array4).
+qed.
+
+(** step 5 : add_and_double **)
+equiv eq_h4_add_and_double_ref4 :
+    MHop2.add_and_double ~ M_ref4.__add_and_double4:
+        init{1} = inzpRep4 init{2}     /\
+        x2{1}   = inzpRep4 x2{2}       /\
+        z2{1}   = inzpRep4 z2r{2}      /\
+        x3{1}   = inzpRep4 x3{2}       /\
+        z3{1}   = inzpRep4 z3{2}
+        ==>
+        res{1}.`1 = inzpRep4 res{2}.`1 /\
+        res{1}.`2 = inzpRep4 res{2}.`2 /\
+        res{1}.`3 = inzpRep4 res{2}.`3 /\
+        res{1}.`4 = inzpRep4 res{2}.`4.
+proof.
+    proc => /=.
+    call eq_h4_mul_rss_ref4.
+    call eq_h4_mul_sss_ref4.
+    call eq_h4_add_sss_ref4.
+    call eq_h4_sqr_ss__ref4.
+    call eq_h4_mul_a24_ss_ref4.
+    call eq_h4_sqr_ss__ref4.
+    call eq_h4_sub_sss_ref4.
+    call eq_h4_mul_sss_ref4.
+    call eq_h4_sub_sss_ref4.
+    call eq_h4_add_sss_ref4.
+    call eq_h4_sqr_ss__ref4.
+    call eq_h4_sqr_ss__ref4.
+    call eq_h4_mul_sss_ref4.
+    call eq_h4_mul_sss_ref4.
+    call eq_h4_add_sss_ref4.
+    call eq_h4_sub_sss_ref4.
+    call eq_h4_add_ssr_ref4.
+    call eq_h4_sub_ssr_ref4.
+    wp. done.
+qed.
+
+(** step 6 : montgomery_ladder_step **)
+equiv eq_h4_montgomery_ladder_step_ref4 :
+    MHop2.montgomery_ladder_step ~ M_ref4.__montgomery_ladder_step4:
+        inzp (to_uint k'{1}) =   inzpRep32 k{2} /\
+        init'{1} = inzpRep4 init{2}             /\
+        x2{1} = inzpRep4 x2{2}                  /\
+        z2{1} = inzpRep4 z2r{2}                 /\
+        x3{1} = inzpRep4 x3{2}                  /\
+        z3{1} = inzpRep4 z3{2}                  /\ 
+        b2i swapped{1} = to_uint swapped{2}     /\
+        ctr'{1} = to_uint ctr{2}
+        ==>
+        res{1}.`1 = inzpRep4 res{2}.`1          /\
+        res{1}.`2 = inzpRep4 res{2}.`2          /\
+        res{1}.`3 = inzpRep4 res{2}.`3          /\
+        res{1}.`4 = inzpRep4 res{2}.`4          /\
+        b2i res{1}.`5 = to_uint res{2}.`5.
+proof.
+    proc => /=. 
+    call eq_h4_add_and_double_ref4. wp.
+    call eq_h4_cswap_ref4. wp.
+    call eq_h4_ith_bit_ref4. skip. 
+    move => &1 &2 [H0] [H1] [H2] [H3] [H4] [H5] [H6] H7. split.   
+    auto => />. rewrite H0. 
+    move => [H8 H9] H10 H11 H12 H13 H14. 
+    split;  auto => />. rewrite /H14 /H13. 
+    rewrite /b2i. 
+    case: (swapped{1} ^^ H10).
+    move => *. smt(@W64). 
+    move => *. smt(@W64). 
+qed.   
+
+(** step 7 : montgomery_ladder **)
+equiv eq_h4_montgomery_ladder_ref4 :
+    MHop2.montgomery_ladder ~ M_ref4.__montgomery_ladder4 :
+        init'{1} = inzpRep4 u{2}                     /\
+        inzp (W256.to_uint k'{1}) =  inzpRep32 k{2}
+        ==>
+        res{1}.`1 = inzpRep4 res{2}.`1               /\
+        res{1}.`2 =inzpRep4  res{2}.`2.
+proof.
+    proc. wp. sp. 
+    unroll {1} 4. 
+    rcondt {1} 4. auto => />. inline MHop2.init_points.
+        wp. sp. skip. auto => />.
+    while(
+          inzp (to_uint k'{1}) = inzpRep32 k{2}            /\ 
+          ctr{1} = to_uint ctr{2}                          /\ 
+          inzp (to_uint k'{1}) = inzpRep32 k{2}            /\
+          init'{1} = inzpRep4 us{2}                        /\ 
+          x2{1} = inzpRep4 x2{2}                           /\
+          x3{1} = inzpRep4 x3{2}                           /\
+          z2{1} = inzpRep4 z2r{2}                          /\
+          z3{1} = inzpRep4 z3{2}                           /\
+          b2i swapped{1} = to_uint swapped{2}).
+        wp. sp. call eq_h4_montgomery_ladder_step_ref4. skip. auto => />. 
+        move => &1 &2 ctrR H H0 H1 H2. split.
+        rewrite to_uintB. rewrite uleE to_uint1 => />. smt(). rewrite to_uint1 => />.
+        move => H3 H4 H5 H6 H7 H8 H9 H10. split.
+        rewrite ultE to_uintB. rewrite uleE to_uint1. smt().
+        rewrite to_uint1 to_uint0. trivial. smt(@W64).  
+    call eq_h4_montgomery_ladder_step_ref4. wp. call eq_h4_init_points_ref4. skip. done.
+qed.
+
+(** step 8 : iterated square **)
+equiv eq_h4_it_sqr_ref4 :
+    MHop2.it_sqr ~ M_ref4._it_sqr4_p:
+        f{1}            =    inzpRep4 x{2} /\
+        i{1}            =    to_uint i{2}  /\
+        2               <=   to_uint i{2}  /\
+        i{1}            <=   W32.modulus   /\
+        2               <=   i{1}   
+        ==>
+        res{1} = inzpRep4 res{2}.
+proof.
+    proc. simplify. wp. sp.
+    while (h{1}            =    inzpRep4 x{2}            /\ 
+         ii{1}            =    to_uint i{2}              /\
+         ii{1}            <=   W32.modulus               /\
+         0                <=   ii{1}                     
+    ).
+    wp. call eq_h4_sqr_p_ref4. conseq(_: _ ==> h{1} = inzpRep4 x{2}).
+    move => &1 &2 [[H][ H0] [H1] H2 [H3] H4 H5]. split. apply H5.
+    rewrite /DEC_32 /rflags_of_aluop_nocf_w /ZF_of => /=.
+    move => H6 H7 H8 H9. split. split. apply H9. split.
+    rewrite to_uintB. rewrite  uleE => />. by smt(). rewrite to_uint1 H0 //.
+    split. move: H1. smt(). move: H2. smt(). split. rewrite H0. move => H10.
+    smt(@W32). smt(@W32). skip. auto => />. wp.
+    rewrite /DEC_32 /rflags_of_aluop_nocf_w /ZF_of => /=. 
+    call eq_h4_sqr_p_ref4.  
+    skip. auto => />. move => &2 H H0. split. split.
+    rewrite to_uintB. rewrite uleE => />. move: H. smt().
+    rewrite to_uint1 //. split. move: H0. smt(). move: H. smt().
+    split. move => H1. smt(@W32). move => H1. move: H. smt().
+qed.
+
+equiv eq_h4_it_sqr_s_ref4 :
+    MHop2.it_sqr ~ M_ref4._it_sqr4_s_:
+        f{1}            =    inzpRep4 x{2} /\
+        i{1}            =    to_uint i{2}  /\
+        2               <=   to_uint i{2}  /\
+        i{1}            <=   W32.modulus   /\
+        2              <=   i{1}   ==>
+        res{1} = inzpRep4 res{2}.
+proof.
+    proc *. inline M_ref4._it_sqr4_s_. wp. sp. 
+    call eq_h4_it_sqr_ref4. skip. auto => />.
+qed.
+
+equiv eq_h4_it_sqr_ss_ref4 :
+        MHop2.it_sqr ~ M_ref4._it_sqr4_ss_: 
+        f{1}            =    inzpRep4 x{2} /\
+        i{1}            =    to_uint i{2}  /\
+        2               <=   to_uint i{2}  /\
+        i{1}            <=   W32.modulus   /\
+        2               <=   i{1}   
+        ==>
+        res{1} = inzpRep4 res{2}.
+proof.
+    proc *. inline M_ref4._it_sqr4_ss_. 
+    unroll for{2} ^while. wp. sp.
+    call eq_h4_it_sqr_ref4. skip. auto => />. move => &2 H H0. congr. 
+    apply Array4.ext_eq. move => H1 [H2] H3. smt(@Array4).
+qed.
+
+(** step 9 : invert **)
+equiv eq_h4_invert_ref4 :
+    MHop2.invert ~ M_ref4.__invert4 : 
+        fs{1} = inzpRep4 fs{2}
+        ==> 
+        res{1} = inzpRep4 res{2}.
+proof.
+    proc.
+    sp.
+    call eq_h4_mul_ss_ref4.
+    call eq_h4_sqr_s__ref4.
+    call (eq_h4_it_sqr_s_ref4). wp.
+    call eq_h4_mul_ss_ref4.
+    call eq_h4_it_sqr_s_ref4. wp.
+    call eq_h4_mul_ss_ref4.
+    call eq_h4_it_sqr_ss_ref4. wp.
+    call eq_h4_mul_ss_ref4.
+    call eq_h4_it_sqr_ss_ref4. wp.
+    call eq_h4_mul_ss_ref4.
+    call eq_h4_it_sqr_s_ref4. wp.
+    call eq_h4_mul_ss_ref4.
+    call eq_h4_it_sqr_ss_ref4. wp.
+    call eq_h4_mul_ss_ref4.
+    call eq_h4_it_sqr_ss_ref4. wp.
+    call eq_h4_mul_ss_ref4.
+    call eq_h4_it_sqr_s_ref4. wp.
+    call eq_h4_sqr_ss_ref4.
+    call eq_h4_mul_ss_ref4.
+    call eq_h4_sqr_ss_ref4.
+    call eq_h4_mul_ss_ref4.
+    call eq_h4_mul_ss_ref4.
+    call eq_h4_sqr_s__ref4.
+    call eq_h4_sqr_ss_ref4.
+    call eq_h4_sqr_ss_ref4. wp. 
+    skip. done.
+qed.
+
+
+(** step 11 : scalarmult **)
+
+equiv eq_h4_scalarmult_internal_ref4 :
+    MHop2.scalarmult_internal ~ M_ref4.__curve25519_internal_ref4:
+        inzp(W256.to_uint k'{1}) = inzpRep32 k{2} /\  
+        u''{1} = inzpRep4 u{2}
+        ==>
+        inzp(W256.to_uint res{1}) = inzpRep4 res{2}. 
+proof.
+    proc.
+    call eq_h4_encode_point_ref4.
+    call eq_h4_montgomery_ladder_ref4. wp. skip.
+    done.
+qed.
+
+equiv eq_h4_scalarmult_ref4 :
+    MHop2.scalarmult ~ M_ref4._curve25519_ref4:
+        inzp(W256.to_uint k'{1}) = inzpRep4 _k{2} /\  
+        inzp (to_uint u'{1}) = inzpRep4 _u{2}
+        ==>
+        inzp(W256.to_uint res{1}) = inzpRep4 res{2} /\
+        inzpRep32List (W32u8.to_list res{1}) = inzpRep4 res{2}.
+proof.
+    proc.
+    call eq_h4_scalarmult_internal_ref4 => />. auto => />.
+    move => &1 &2 H H0 H1 H2 H3 H4 H5 H6 H7. auto => />.
+    rewrite -H7.
+    rewrite /inzpRep32List /inzpRep4 /valRep32List. congr. 
+    rewrite to_uint_unpack32u8. congr. congr. smt().
+    call eq_h4_decode_u_coordinate_ref4 => />.
+    call eq_h4_decode_scalar_25519_ref4 => />.
+    move => &1 &2 [H] H0 H1. split. auto => />.
+    move => H2 H3 H4 H5 H6. split. auto => />.
+    move => H7 H8 H9 H10. rewrite -H10.
+    rewrite /inzpRep32List /inzpRep4 /valRep32List. congr.
+    rewrite to_uint_unpack32u8. congr. congr. smt().
+    wp. skip. 
+    auto => />. move => &1 &2 H H0 H1 H2 H3 H4 H5 H6.
+    rewrite -H6.
+    rewrite /inzpRep32List /inzpRep4 /valRep32List. congr.
+    rewrite to_uint_unpack32u8. congr. congr. smt().
+qed.
+
+
+lemma eq_h4_scalarmult_ptr_ref4 mem _rp _kp _up :
+    equiv [MHop2.scalarmult ~ M_ref4.__curve25519_ref4_ptr:
+        valid_ptr (W64.to_uint _up)  32                                                          /\ 
+        valid_ptr (W64.to_uint _kp)  32                                                          /\
+        valid_ptr (W64.to_uint _rp)  32                                                          /\
+        Glob.mem{2} = mem                                                                        /\
+        rp{2} = _rp                                                                              /\ 
+        kp{2} = _kp                                                                              /\
+        up{2} = _up                                                                              /\ 
+        inzp (W256.to_uint u'{1}) = inzpRep4List (load_array4 (mem) (W64.to_uint _up))           /\
+        inzp (W256.to_uint k'{1}) = inzpRep4List (load_array4 (mem) (W64.to_uint _kp))             
+        ==>
+        inzpRep32List(W32u8.to_list res{1}) = inzpRep4List (load_array4 Glob.mem{2} (W64.to_uint _rp))    /\
+        res{2} = tt
+    ].
+proof.
+    proc *.
+    inline M_ref4.__curve25519_ref4_ptr. wp. sp.
+    inline M_ref4.__load4 M_ref4.__store4. 
+    do 3! unroll for{2} ^while.
+    sp. wp. auto => />.
+    call eq_h4_scalarmult_ref4. skip. auto => />.
+    move => &1 &2 H H0 H1 H2 H3 H4 H5 H6. 
+    split. split.
+    rewrite H6 /inzpRep4List /inzpRep4 /valRep4 /valRep4List /load_array4.
+    congr. congr. congr. rewrite /to_list /mkseq -iotaredE. auto => />.  
+    rewrite !to_uintD_small !to_uint_small => />. 
+    move: H2. smt(). move: H1. smt(). move: H2. smt().
+    rewrite H5 /inzpRep4List /inzpRep4 /valRep4 /valRep4List /load_array4.
+    congr. congr. congr. rewrite /to_list /mkseq -iotaredE. auto => />.  
+    rewrite !to_uintD_small !to_uint_small => />. 
+    move: H5. smt(). move: H5. smt(). move: H5. smt().
+    move => H7 H8 H9 H10 H11. auto => />. rewrite -H11.
+    move => H12. rewrite H12 H11.
+    rewrite /inzpRep4List /inzpRep4 /valRep4 /valRep4List /load_array4.
+    congr. congr. congr. rewrite /to_list /mkseq -iotaredE => />. 
+    split. apply (load_store_pos Glob.mem{2} rp{2} H10 0). 
+    rewrite /valid_ptr. split. trivial. apply H4. trivial.
+    split. apply (load_store_pos Glob.mem{2} rp{2} H10 8). 
+    rewrite /valid_ptr. split. trivial. apply H4. trivial.
+    split. apply (load_store_pos Glob.mem{2} rp{2} H10 16). 
+    rewrite /valid_ptr. split. trivial. apply H4. trivial.
+    apply (load_store_pos Glob.mem{2} rp{2} H10 24). 
+    rewrite /valid_ptr. split. trivial. apply H4. trivial.    
+qed.
+
+
+equiv eq_h4_scalarmult_base_ref4 :
+    MHop2.scalarmult_base ~ M_ref4._curve25519_ref4_base:
+        inzp(W256.to_uint k'{1}) = inzpRep4 _k{2} 
+        ==>  
+        inzp(W256.to_uint res{1}) = inzpRep4 res{2}. 
+proof.
+    proc.
+    call eq_h4_scalarmult_internal_ref4 => />.
+    call eq_h4_decode_u_coordinate_base_ref4 => />.
+    call eq_h4_decode_scalar_25519_ref4.
+    wp. skip. done.
+qed.
+
+
+lemma eq_h4_scalarmult_base_ptr_ref4 mem _rp _kp : 
+ equiv [MHop2.scalarmult_base ~ M_ref4.__curve25519_ref4_base_ptr:
+        valid_ptr (W64.to_uint _rp) 32 /\
+        valid_ptr (W64.to_uint _kp) 32 /\
+        Glob.mem{2} = mem /\
+        rp{2} = _rp /\
+        kp{2} = _kp /\
+        inzp(W256.to_uint k'{1}) = inzpRep4List (load_array4 (Glob.mem{2}) (W64.to_uint _kp))
+        ==>
+        inzp(W256.to_uint res{1}) = inzpRep4List (load_array4 Glob.mem{2} (W64.to_uint _rp)) /\ res{2} = tt].
+proof.
+    proc *. inline M_ref4.__curve25519_ref4_base_ptr M_ref4.__load4 M_ref4.__store4. 
+    do 2! unroll for{2} ^while. wp. sp. call eq_h4_scalarmult_base_ref4.
+    skip. auto => />.  move => &1 &2 H H0 H1 H2. split.
+    rewrite H2. rewrite /inzpRep4List /inzpRep4 /valRep4 /valRep4List /load_array4 /to_list /mkseq -iotaredE.
+    congr. congr. congr. auto => />. rewrite !to_uintD_small !to_uint_small; smt(); smt().    
+    move => H3 H4 H5 H6. rewrite H6. rewrite /inzpRep4 /inzpRep4List /valRep4 /valRep4List.
+    congr. congr. congr. rewrite /to_list /mkseq /load_array4 -iotaredE => />. split.
+    apply (load_store_pos mem _rp H5 0). rewrite /valid_ptr. smt(). smt(). split.
+    apply (load_store_pos mem _rp H5 8). rewrite /valid_ptr. smt(). smt(). split.
+    apply (load_store_pos mem _rp H5 16). rewrite /valid_ptr. smt(). smt(). 
+    apply (load_store_pos mem _rp H5 24). rewrite /valid_ptr. smt(). smt().
+qed.    
+
+
+lemma eq_h4_scalarmult_jade_ref4 mem _qp _np _pp:
+    equiv [MHop2.scalarmult ~ M_ref4.jade_scalarmult_curve25519_amd64_ref4:
+        valid_ptr (W64.to_uint _qp)  32                                                          /\ 
+        valid_ptr (W64.to_uint _np)  32                                                          /\
+        valid_ptr (W64.to_uint _pp)  32                                                          /\
+        Glob.mem{2} = mem                                                                        /\
+        qp{2} = _qp                                                                              /\ 
+        np{2} = _np                                                                              /\
+        pp{2} = _pp                                                                              /\ 
+        inzp (W256.to_uint k'{1}) = inzpRep4List (load_array4 (Glob.mem{2}) (W64.to_uint np{2})) /\  
+        inzp (to_uint u'{1})      = inzpRep4List (load_array4 (Glob.mem{2}) (W64.to_uint pp{2}))
+        ==>
+        inzp(W256.to_uint res{1}) = inzpRep4List (load_array4 Glob.mem{2} (W64.to_uint _qp))     /\
+        res{2} = W64.zero].
+proof.
+    proc *. inline M_ref4.jade_scalarmult_curve25519_amd64_ref4. wp. sp.
+    call (eq_h4_scalarmult_ptr_ref4 mem _qp _np _pp). skip. auto => />.
+    move => &1 H H0 H1 H2 H3 H4 H5 H6 H7 H8 H9.
+    rewrite -H9. rewrite to_uint_unpack32u8. rewrite /inzpRep32List /valRep32List.
+    congr. congr. congr. smt(@W32u8).
+qed.
+
+
+lemma eq_h4_scalarmult_jade_base_ref4  mem _qp _np:
+    equiv [MHop2.scalarmult_base ~ M_ref4.jade_scalarmult_curve25519_amd64_ref4_base:
+        valid_ptr (W64.to_uint _qp)  32                                                          /\ 
+        valid_ptr (W64.to_uint _np)  32                                                          /\
+        Glob.mem{2} = mem                                                                        /\
+        qp{2} = _qp                                                                              /\ 
+        np{2} = _np                                                                              /\
+        inzp (W256.to_uint k'{1}) = inzpRep4List (load_array4 (Glob.mem{2}) (W64.to_uint np{2}))  
+        ==>
+        inzp(W256.to_uint res{1}) = inzpRep4List (load_array4 Glob.mem{2} (W64.to_uint _qp))     /\
+        res{2} = W64.zero].
+proof.
+    proc *. inline M_ref4.jade_scalarmult_curve25519_amd64_ref4_base. wp. sp.
+    call (eq_h4_scalarmult_base_ptr_ref4 mem _qp _np). skip. done.
+qed.
+
+
+
