src/ref4/Curve25519_auto4.ec
@@ -1,0 +1,257 @@
+require import Int Bool Zp_25519 List.
+require import Curve25519_Spec.
+require import Curve25519_Hop1.
+require import Curve25519_Hop2.
+require import Curve25519_Ref4.
+require import W64limbs.
+
+from Jasmin require import JWord JWord_array.
+
+import Zp_25519 Curve25519_Spec Curve25519_Hop2 Curve25519_Ref4 Array4 Array32.
+
+(* Probably needs to be moved elsewhere, such as W64limbs *)
+
+(** step 0 : add sub mul sqr - all done by auto **)
+
+equiv eq_h4_add : MHop2.add ~ M_ref4.__add4_rrs:
+    f{1}   = inzpRep4 f{2} /\
+    g{1}   = inzpRep4 g{2}
+    ==>
+    res{1} = inzpRep4 res{2}.
+proof. 
+    proc.  
+    admit.
+qed.
+
+equiv eq_h4_sub_ref4 : MHop2.sub ~ M_ref4.__sub4_rrs:
+   f{1}   = inzpRep4 f{2} /\
+   g{1}   = inzpRep4 gs{2}
+   ==>
+   res{1} = inzpRep4 res{2}.
+proof.
+    proc.
+    admit.
+qed.
+
+equiv eq_h4_mul_a24_ref4 : MHop2.mul_a24 ~ M_ref4.__mul4_a24_rs:
+    f{1}   = inzpRep4 xa{2} /\
+    a24{1} = to_uint a24{2}
+    ==>
+    res{1} = inzpRep4 res{2}.
+proof.
+    proc.
+    admit.
+qed.
+
+equiv eq_h4_mul_rss_ref4 : MHop2.mul ~ M_ref4.__mul4_rss:
+    f{1}   = inzpRep4 xa{2} /\
+    g{1}   = inzpRep4 ya{2}
+    ==>
+    res{1} = inzpRep4 res{2}.
+proof.
+    proc.
+    admit.
+qed.
+
+equiv eq_h4_sqr_ref4 : MHop2.sqr ~ M_ref4.__sqr4_rs:
+    f{1}   = inzpRep4 xa{2}
+    ==>
+    res{1} = inzpRep4 res{2}.
+proof.
+    proc.
+    admit.
+qed.
+
+(** step 0.5 : transitivity stuff **)
+equiv eq_h4_add_ssr_ref4 : MHop2.add ~ M_ref4.__add4_ssr:
+    f{1}   = inzpRep4 fs{2} /\
+    g{1}   = inzpRep4 g{2}
+    ==>
+    res{1} = inzpRep4 res{2}.
+proof.
+    proc.
+    admit.
+qed.
+
+
+equiv eq_h4_add_sss_ref4 : MHop2.add ~ M_ref4.__add4_sss:
+    f{1}   = inzpRep4 fs{2} /\
+    g{1}   = inzpRep4 gs{2}
+    ==>
+    res{1} = inzpRep4 res{2}.
+proof.
+    proc.
+    admit.
+qed.
+
+equiv eq_h4_add_rrs_ref4 : MHop2.add ~ M_ref4.__add4_rrs:
+    f{1}   = inzpRep4 f{2} /\
+    g{1}   = inzpRep4 g{2}
+    ==>
+    res{1} = inzpRep4 res{2}.
+proof.
+    proc.
+    admit.
+qed.
+
+
+equiv eq_h4_sub_ssr_ref4 : MHop2.sub ~ M_ref4.__sub4_ssr:
+    f{1} = inzpRep4 fs{2} /\
+    g{1} = inzpRep4 g{2}
+    ==>
+    res{1} = inzpRep4 res{2}.
+proof.
+    proc.
+    admit.
+qed.
+
+equiv eq_h4_sub_rsr_ref4 : MHop2.sub ~ M_ref4.__sub4_rsr:
+    f{1}   = inzpRep4 fs{2} /\
+    g{1}   = inzpRep4 g{2}
+    ==>
+    res{1} = inzpRep4 res{2}.
+proof.
+    proc.
+    admit.
+qed.
+
+equiv eq_h4_sub_sss_ref4 : MHop2.sub ~ M_ref4.__sub4_sss:
+    f{1}   = inzpRep4 fs{2} /\
+    g{1}   = inzpRep4 gs{2}
+    ==>
+    res{1} = inzpRep4 res{2}.
+proof.
+    proc.
+    admit.
+qed.
+
+equiv eq_h4_mul_a24_ss_ref4 : MHop2.mul_a24 ~ M_ref4.__mul4_a24_ss:
+    f{1}   = inzpRep4 xa{2} /\
+    a24{1} = to_uint a24{2}
+    ==>
+    res{1} = inzpRep4 res{2}.
+proof.
+    proc.
+    admit.
+qed.
+
+equiv eq_h4_mul_sss_ref4 : MHop2.mul ~ M_ref4.__mul4_sss:
+    f{1}   = inzpRep4 xa{2} /\
+    g{1}   = inzpRep4 ya{2}
+    ==>
+    res{1} = inzpRep4 res{2}.
+proof.
+    proc.
+    admit.
+qed.
+
+equiv eq_h4_mul_pp_ref4 : MHop2.mul ~ M_ref4._mul4_pp:
+    f{1}   = inzpRep4 xa{2} /\
+    g{1}   = inzpRep4 ya{2}
+    ==>
+    res{1} = inzpRep4 res{2}.
+proof.
+    proc.
+    admit.
+qed.
+
+
+equiv eq_h4_mul_ss_ref4 : MHop2.mul ~ M_ref4._mul4_ss_:
+    f{1}   = inzpRep4 xa{2} /\
+    g{1}   = inzpRep4 ya{2}
+    ==>
+    res{1} = inzpRep4 res{2}.
+proof.
+    proc.
+    admit.
+qed.
+
+
+equiv eq_h4_sqr_rs_ref4 : MHop2.sqr ~ M_ref4.__sqr4_rs:
+    f{1}   = inzpRep4 xa{2}
+    ==>
+    res{1} = inzpRep4 res{2}.
+proof.
+    proc.
+    admit.
+qed.
+
+equiv eq_h4_sqr_ss_ref4 : MHop2.sqr ~ M_ref4._sqr4_ss_:
+    f{1} = inzpRep4 xa{2}
+    ==>
+    res{1} = inzpRep4 res{2}.
+proof.
+    proc.
+    admit.
+qed.
+
+equiv eq_h4_sqr_ss__ref4 : MHop2.sqr ~ M_ref4.__sqr4_ss:
+    f{1}   = inzpRep4 xa{2}
+    ==>
+    res{1} = inzpRep4 res{2}.
+proof.
+    proc.
+    admit.
+qed.
+
+equiv eq_h4_sqr_s__ref4 : MHop2.sqr ~ M_ref4._sqr4_s_:
+    f{1}   = inzpRep4 x{2}
+    ==>
+    res{1} = inzpRep4 res{2}.
+proof.
+    proc.
+    admit.
+qed.
+
+equiv eq_h4_sqr_p_ref4 : MHop2.sqr ~ M_ref4._sqr4_p:
+    f{1}   = inzpRep4 xa{2}
+    ==>
+    res{1} = inzpRep4 res{2}.
+proof.
+    proc.
+    admit.
+qed.
+
+
+(** step 1 : decode_scalar_25519 **)
+equiv eq_h4_decode_scalar_25519_ref4 : MHop2.decode_scalar ~ M_ref4.__decode_scalar:
+    inzp (W256.to_uint k'{1})  = inzpRep4 k{2}
+    ==> 
+    inzp (W256.to_uint res{1}) = inzpRep32 res{2}. 
+proof.
+    admit. (* AUTO *)
+qed.
+
+
+(** step 2 : decode_u_coordinate **)
+equiv eq_h4_decode_u_coordinate_ref4 : MHop2.decode_u_coordinate ~ M_ref4.__decode_u_coordinate4:
+    inzp (W256.to_uint u'{1}) = inzpRep4 u{2}
+    ==> 
+    res{1}                    = inzpRep4 res{2}.
+proof.
+    admit. (* AUTO MSB already 0 -  ask tiago *)
+qed.
+
+(** step 3 : ith_bit **)
+equiv eq_h4_ith_bit_ref4 : MHop2.ith_bit ~ M_ref4.__ith_bit :
+    inzp (W256.to_uint k'{1}) = inzpRep32 k{2} /\  
+    (ctr{1}                   = to_uint ctr{2}) 
+    ==> 
+    b2i res{1}                = to_uint res{2}.
+proof.
+    proc.
+    admit. (* AUTO *)
+qed.
+
+
+(** step 10 : encode point **)
+equiv eq_h4_encode_point_ref4 : MHop2.encode_point ~ M_ref4.__encode_point4:
+    x2{1}                 = inzpRep4 x2{2} /\ 
+    z2{1}                 = inzpRep4 z2r{2}
+    ==>
+    inzp (to_uint res{1}) = inzpRep4 res{2}.
+proof.
+    admit. (* AUTO *)
+qed.
+    
+
