src/ref5/Curve25519_auto5.ec
@@ -1,0 +1,221 @@
+require import Int Bool Zp_25519 List.
+require import Curve25519_Spec.
+require import Curve25519_Hop1.
+require import Curve25519_Hop2.
+require import Curve25519_Ref5.
+require import W64limbs.
+
+from Jasmin require import JWord JWord_array.
+
+import Zp_25519 Curve25519_Spec Curve25519_Hop2 Curve25519_Ref5 Array4 Array32 Array5.
+
+(** ref5 **)
+
+
+
+equiv eq_h4_add_rrs_ref5 : MHop2.add ~ M_ref5.__add5_rrs:
+   f{1}   = inzpRep5 f{2} /\
+   g{1}   = inzpRep5 g{2}
+   ==>
+   res{1} = inzpRep5 res{2}.
+proof.
+    proc.
+    admit.
+qed.
+
+equiv eq_h4_add_sss_ref5 : MHop2.add ~ M_ref5.__add5_sss:
+   f{1}   = inzpRep5 fs{2} /\
+   g{1}   = inzpRep5 gs{2}
+   ==>
+   res{1} = inzpRep5 res{2}.
+proof.
+    proc.
+    admit.
+qed.
+
+equiv eq_h4_add_ssr_ref5 : MHop2.add ~ M_ref5.__add5_ssr:
+   f{1}   = inzpRep5 fs{2} /\
+   g{1}   = inzpRep5 g{2}
+   ==>
+   res{1} = inzpRep5 res{2}.
+proof.
+    proc.
+    admit.
+qed.
+
+
+
+equiv eq_h4_sub_rss_ref5 : MHop2.sub ~ M_ref5.__sub5_rrs:
+   f{1}   = inzpRep5 f{2} /\
+   g{1}   = inzpRep5 gs{2}
+   ==>
+   res{1} = inzpRep5 res{2}.
+proof.
+    proc.
+    admit.
+qed.
+
+
+equiv eq_h4_sub_sss_ref5 : MHop2.sub ~ M_ref5.__sub5_sss:
+   f{1}   = inzpRep5 fs{2} /\
+   g{1}   = inzpRep5 gs{2}
+   ==>
+   res{1} = inzpRep5 res{2}.
+proof.
+    proc.
+    admit.
+qed.
+
+
+equiv eq_h4_sub_rsr_ref5 : MHop2.sub ~ M_ref5.__sub5_rsr:
+   f{1}   = inzpRep5 fs{2} /\
+   g{1}   = inzpRep5 g{2}
+   ==>
+   res{1} = inzpRep5 res{2}.
+proof.
+    proc.
+    admit.
+qed.
+
+
+equiv eq_h4_sub_ssr_ref5 : MHop2.sub ~ M_ref5.__sub5_ssr:
+   f{1}   = inzpRep5 fs{2} /\
+   g{1}   = inzpRep5 g{2}
+   ==>
+   res{1} = inzpRep5 res{2}.
+proof.
+    proc.
+    admit.
+qed.
+
+
+equiv eq_h4_mul_rss_ref5 : MHop2.mul ~ M_ref5.__mul5_rss:
+    f{1}   = inzpRep5 xa{2} /\
+    g{1}   = inzpRep5 ya{2}
+    ==>
+    res{1} = inzpRep5 res{2}.
+proof.
+    proc.
+    admit.
+qed.
+
+
+equiv eq_h4_mul_sss_ref5 : MHop2.mul ~ M_ref5.__mul5_sss:
+    f{1}   = inzpRep5 xa{2} /\
+    g{1}   = inzpRep5 ya{2}
+    ==>
+    res{1} = inzpRep5 res{2}.
+proof.
+    proc.
+    admit.
+qed.
+
+
+equiv eq_h4_mul_pp_ref5 : MHop2.mul ~ M_ref5._mul5_pp:
+    f{1}   = inzpRep5 xa{2} /\
+    g{1}   = inzpRep5 ya{2}
+    ==>
+    res{1} = inzpRep5 res{2}.
+proof.
+    proc.
+    admit.
+qed.
+
+equiv eq_h4_mul_ss_ref5 : MHop2.mul ~ M_ref5._mul5_ss_:
+    f{1}   = inzpRep5 xa{2} /\
+    g{1}   = inzpRep5 ya{2}
+    ==>
+    res{1} = inzpRep5 res{2}.
+proof.
+    proc.
+    admit.
+qed.
+
+equiv eq_h4_sqr_rs_ref5 : MHop2.sqr ~ M_ref5.__sqr5_rs:
+    f{1}   = inzpRep5 xa{2}
+    ==>
+    res{1} = inzpRep5 res{2}.
+proof.
+    proc.
+    admit.
+qed.
+
+equiv eq_h4_sqr_ss_ref5 : MHop2.sqr ~ M_ref5.__sqr5_ss:
+    f{1}   = inzpRep5 xa{2}
+    ==>
+    res{1} = inzpRep5 res{2}.
+proof.
+    proc.
+    admit.
+qed.
+
+equiv eq_h4_sqr_p_ref5 : MHop2.sqr ~ M_ref5._sqr5_p:
+    f{1}   = inzpRep5 xa{2}
+    ==>
+    res{1} = inzpRep5 res{2}.
+proof.
+    proc.
+    admit.
+qed.
+
+
+equiv eq_h4_sqr_ss__ref5 : MHop2.sqr ~ M_ref5._sqr5_ss_:
+    f{1}   = inzpRep5 xa{2}
+    ==>
+    res{1} = inzpRep5 res{2}.
+proof.
+    proc.
+    admit.
+qed.
+
+
+equiv eq_h4_sqr_s_ref5 : MHop2.sqr ~ M_ref5._sqr5_s_:
+    f{1}   = inzpRep5 x{2}
+    ==>
+    res{1} = inzpRep5 res{2}.
+proof.
+    proc.
+    admit.
+qed.
+
+
+(** step 1_ref5 : decode_scalar_25519 **)
+equiv eq_h4_decode_scalar_25519_ref5 : MHop2.decode_scalar ~ M_ref5.__decode_scalar:
+    inzp (W256.to_uint k'{1})  = inzpRep4 k{2}
+    ==> 
+    inzp (W256.to_uint res{1}) = inzpRep32 res{2}. 
+proof.
+    admit. (* AUTO *)
+qed.
+
+
+(** step 2_ref5 : decode_u_coordinate **)
+equiv eq_h4_decode_u_coordinate_ref5 : MHop2.decode_u_coordinate ~ M_ref5.__decode_u_coordinate5:
+    inzp (W256.to_uint u'{1}) = inzpRep4 t{2}
+    ==> 
+    res{1}                    = inzpRep5 res{2}.
+proof.
+    admit. (* AUTO MSB already 0 -  ask tiago *)
+qed.
+
+(** step 3_ref5 : ith_bit **)
+equiv eq_h4_ith_bit_ref5 : MHop2.ith_bit ~ M_ref5.__ith_bit:
+    inzp (W256.to_uint k'{1}) = inzpRep32 k{2} /\  
+    (ctr{1}                   = to_uint ctr{2}) 
+    ==> 
+    b2i res{1}                = to_uint res{2}.
+proof.
+    proc.
+    admit. (* AUTO *)
+qed.
+
+
+(** step 10_ref5 : encode point **)
+equiv eq_h4_encode_point_ref5 : MHop2.encode_point ~ M_ref5.__encode_point5:
+    x2{1}                 = inzpRep5 x2{2} /\ 
+    z2{1}                 = inzpRep5 z2r{2}
+    ==>
+    inzp (to_uint res{1}) = inzpRep4 res{2}.
+proof.
+    admit. (* AUTO *)
+qed.
