README.md
@@ -3,15 +3,29 @@ Bringing some libjc X25519 Jasmin-Easycrypt proofs up-to-date (WIP).
 
 Below are files that run without errors as of latest commit date and time and do not include any `admit.` or `smt.`. 
 
+
+### Common
 - [X] EClib.ec 
 - [X] W64limbs.ec 
 - [X] Zp_25519.ec
-- [X] Curve25519_auto.ec
-    - Everything that is to be proven in Cryptoline, hence all lemmas are admitted for now.
 - [X] Curve25519_spec.ec
 - [X] Curve25519_Hop1.ec
 - [X] Curve25519_Hop2.ec 
 - [X] Curve25519_Hop3.ec
+
+### Ref4
 - [X] Curve25519_Hop4.ec
+- [X] Curve25519_auto4.ec
+
+### Ref5
+- [X] Curve25519_Hop4.ec
+- [X] Curve25519_auto5.ec
+
+### Mulx
+- [ ] Curve25519_Hop4.ec 
+    - Invert and add_double not done.
+- [X] Curve25519_auto_mulx.ec
+
+Everything that is to be proven in Cryptoline are in the Curve25519_auto* files, Due to this, all lemmas are admitted for now.
 
 The original Easycrypt files can be found [in the x25519 branch in libjc](https://github.com/tfaoliveira/libjc/tree/x25519/proof/crypto_scalarmult/curve25519).
